Platform-independent implementation of Conventions.size_arguments (#222)
The "size_arguments" function and its properties can be systematically
derived from the "loc_arguments" function and its properties.

Before, the RISC-V port used this derivation, and all other ports
used hand-written "size_arguments" functions and proofs.

This commit moves the definition of "size_arguments" to the
platform-independent file backend/Conventions.v, using the systematic
derivation, and removes the platform-specific definitions.

This reduces code and proof size, and makes it easier to change the
calling conventions.

x86/Asmexpand.ml
@@ -251,7 +251,7 @@ let expand_builtin_va_start_32 r =
     invalid_arg "Fatal error: va_start used in non-vararg function";
   let ofs =
     Int32.(add (add !PrintAsmaux.current_function_stacksize 4l)
-               (mul 4l (Z.to_int32 (Conventions1.size_arguments
+               (mul 4l (Z.to_int32 (Conventions.size_arguments
                                       (get_current_function_sig ()))))) in
   emit (Pleal (RAX, linear_addr RSP (Z.of_uint32 ofs)));
   emit (Pmovl_mr (linear_addr r _0z, RAX))
